LeanWang.lean
@@ -4,9 +4,11 @@ import LeanWang.FiniteSearchProgram
 import LeanWang.FuelMachine
 import LeanWang.Machine
 import LeanWang.MachineTiles
+import LeanWang.PostMachine
 import LeanWang.PartrecToTM2Support
 import LeanWang.PartrecToTM2Table
 import LeanWang.ToPartrecEncoding
 import LeanWang.ToPartrecHelpers
 import LeanWang.NatPartrecToToPartrec
+import LeanWang.TM0Route
 import LeanWang.Theorems
